wip

code/bignum/Hacl.Impl.Exponentiation.fst
@@ -14,13 +14,15 @@ module LSeq = Lib.Sequence
 module BSeq = Lib.ByteSequence
 module Loops = Lib.LoopCombinators
 
-module S = Lib.Exponentiation
+module LE = Lib.Exponentiation
+module SE = Spec.Exponentiation
+
 module BD = Hacl.Bignum.Definitions
 module BN = Hacl.Bignum
 module SN = Hacl.Spec.Bignum
 module BB = Hacl.Bignum.Base
-module SB = Hacl.Spec.Bignum.Base
-module PT = Hacl.Spec.PrecompTable
+module PT = Hacl.Impl.PrecompTable
+
 
 #reset-options "--z3rlimit 50 --fuel 0 --ifuel 0"
 
@@ -29,11 +31,11 @@ let lexp_rl_vartime #a_t len ctx_len k ctx a bLen bBits b acc =
   let h0 = ST.get () in
 
   [@inline_let]
-  let refl1 i : GTot (k.to.a_spec & k.to.a_spec) =
+  let refl1 i : GTot (k.to.t_spec & k.to.t_spec) =
     (refl (as_seq h0 acc), refl (as_seq h0 a)) in
 
   [@inline_let]
-  let spec (h:mem) = S.exp_rl_f k.to.comm_monoid (v bBits) (BD.bn_v h0 b) in
+  let spec (h:mem) = SE.exp_rl_f k.to.concr_ops (v bBits) (BD.bn_v h0 b) in
 
   [@inline_let]
   let inv h (i:nat{i <= v bBits}) =
@@ -73,7 +75,7 @@ val cswap2:
   (ensures  fun h0 _ h1 -> modifies (loc p1 |+| loc p2) h0 h1 /\
     k.to.linv (as_seq h1 p1) /\ k.to.linv (as_seq h1 p2) /\
     (k.to.refl (as_seq h1 p1), k.to.refl (as_seq h1 p2)) ==
-    S.cswap (v bit) (k.to.refl (as_seq h0 p1)) (k.to.refl (as_seq h0 p2)))
+    LE.cswap (v bit) (k.to.refl (as_seq h0 p1)) (k.to.refl (as_seq h0 p2)))
 
 let cswap2 #a_t len ctx_len k bit p1 p2 =
   let h0 = ST.get () in
@@ -110,11 +112,11 @@ let lexp_mont_ladder_swap_consttime #a_t len ctx_len k ctx a bLen bBits b acc =
   let h0 = ST.get () in
 
   [@inline_let]
-  let refl1 i : GTot (k.to.a_spec & k.to.a_spec & nat) =
+  let refl1 i : GTot (k.to.t_spec & k.to.t_spec & nat) =
     (k.to.refl (as_seq h0 acc), k.to.refl (as_seq h0 a), v (LSeq.index (as_seq h0 sw) 0)) in
 
   [@inline_let]
-  let spec (h:mem) = S.exp_mont_ladder_swap_f k.to.comm_monoid (v bBits) (BD.bn_v h0 b) in
+  let spec (h:mem) = SE.exp_mont_ladder_swap_f k.to.concr_ops (v bBits) (BD.bn_v h0 b) in
 
   [@inline_let]
   let inv h (i:nat{i <= v bBits}) =
@@ -151,20 +153,18 @@ let lexp_mont_ladder_swap_consttime #a_t len ctx_len k ctx a bLen bBits b acc =
 let lexp_pow_in_place #a_t len ctx_len k ctx acc b =
   let h0 = ST.get () in
   [@ inline_let]
-  let refl1 i : GTot k.to.a_spec = k.to.refl (as_seq h0 acc) in
-  [@ inline_let]
-  let spec h0 = S.sqr k.to.comm_monoid in
+  let refl1 i : GTot k.to.t_spec = k.to.refl (as_seq h0 acc) in
 
   [@ inline_let]
   let inv h (i:nat{i <= v b}) =
     modifies (loc acc) h0 h /\
     k.to.linv (as_seq h acc) /\
-    k.to.refl (as_seq h acc) == Loops.repeat i (spec h0) (refl1 0) in
+    k.to.refl (as_seq h acc) == Loops.repeat i k.to.concr_ops.SE.sqr (refl1 0) in
 
-  Loops.eq_repeat0 (spec h0) (refl1 0);
+  Loops.eq_repeat0 k.to.concr_ops.SE.sqr (refl1 0);
   Lib.Loops.for 0ul b inv
   (fun j ->
-    Loops.unfold_repeat (v b) (spec h0) (refl1 0) (v j);
+    Loops.unfold_repeat (v b) k.to.concr_ops.SE.sqr (refl1 0) (v j);
     k.lsqr ctx acc acc)
 
 
@@ -179,7 +179,7 @@ val precomp_table_inv:
   -> ctx_len:size_t
   -> k:concrete_ops a_t len ctx_len
   -> a:LSeq.lseq (uint_t a_t SEC) (v len)
-  -> table_len:size_t{v table_len * v len <= max_size_t}
+  -> table_len:size_t{1 < v table_len /\ v table_len * v len <= max_size_t}
   -> table:LSeq.lseq (uint_t a_t SEC) (v table_len * v len)
   -> j:nat{j < v table_len} ->
   Type0
@@ -188,155 +188,8 @@ let precomp_table_inv #a_t len ctx_len k a table_len table j =
   Math.Lemmas.lemma_mult_le_right (v len) (j + 1) (v table_len);
   let bj = LSeq.sub table (j * v len) (v len) in
   k.to.linv bj /\ k.to.linv a /\
-  k.to.refl bj == S.pow k.to.comm_monoid (k.to.refl a) j
-
-
-inline_for_extraction noextract
-val lprecomp_table_mul:
-    #a_t:inttype_a
-  -> len:size_t{v len > 0}
-  -> ctx_len:size_t
-  -> k:concrete_ops a_t len ctx_len
-  -> ctx:lbuffer (uint_t a_t SEC) ctx_len
-  -> a:lbuffer (uint_t a_t SEC) len
-  -> i:size_t
-  -> ti:lbuffer (uint_t a_t SEC) len
-  -> res:lbuffer (uint_t a_t SEC) len ->
-  Stack unit
-  (requires fun h ->
-    live h a /\ live h ti /\ live h ctx /\ live h res /\
-    disjoint a ti /\ disjoint a ctx /\ disjoint a res /\
-    disjoint ti ctx /\ disjoint ti res /\ disjoint ctx res /\
-    k.to.linv (as_seq h a) /\ k.to.linv_ctx (as_seq h ctx) /\
-    k.to.linv (as_seq h ti) /\
-    k.to.refl (as_seq h ti) == S.pow k.to.comm_monoid (k.to.refl (as_seq h a)) (v i + 1))
-  (ensures  fun h0 _ h1 -> modifies (loc res) h0 h1 /\
-    k.to.linv (as_seq h1 res) /\
-    k.to.refl (as_seq h1 res) == S.pow k.to.comm_monoid (k.to.refl (as_seq h0 a)) (v i + 2))
-
-let lprecomp_table_mul #a_t len ctx_len k ctx a i ti res =
-  let h0 = ST.get () in
-  k.lmul ctx ti a res;
-  let h1 = ST.get () in
-  assert (k.to.refl (as_seq h1 res) == k.to.comm_monoid.S.mul (k.to.refl (as_seq h0 ti)) (k.to.refl (as_seq h0 a)));
-  S.lemma_pow_add k.to.comm_monoid (k.to.refl (as_seq h0 a)) (v i + 1) 1;
-  S.lemma_pow1 k.to.comm_monoid (k.to.refl (as_seq h0 a))
-
-
-#push-options "--z3rlimit 150"
-inline_for_extraction noextract
-val precomp_table_inv_lemma_j:
-    #a_t:inttype_a
-  -> len:size_t{v len > 0}
-  -> ctx_len:size_t
-  -> k:concrete_ops a_t len ctx_len
-  -> a:LSeq.lseq (uint_t a_t SEC) (v len)
-  -> table_len:size_t{v table_len * v len <= max_size_t}
-  -> table1:LSeq.lseq (uint_t a_t SEC) (v table_len * v len)
-  -> table2:LSeq.lseq (uint_t a_t SEC) (v table_len * v len)
-  -> i:nat{i <= v table_len}
-  -> j:nat{j < i} -> Lemma
-  (requires
-    LSeq.sub table1 0 (i * v len) == LSeq.sub table2 0 (i * v len) /\
-    precomp_table_inv len ctx_len k a table_len table1 j)
-  (ensures
-    precomp_table_inv len ctx_len k a table_len table2 j)
-
-let precomp_table_inv_lemma_j #a_t len ctx_len k a table_len table1 table2 i j =
-  assert (precomp_table_inv len ctx_len k a table_len table1 j);
-  Math.Lemmas.lemma_mult_le_right (v len) (j + 1) (v table_len);
-  let bj1 = LSeq.sub table1 (j * v len) (v len) in
-  let bj2 = LSeq.sub table2 (j * v len) (v len) in
-
-  let aux (l:nat{l < v len}) : Lemma (LSeq.index bj1 l == LSeq.index bj2 l) =
-    Seq.lemma_index_slice table1 (j * v len) (j * v len + v len) l;
-    assert (LSeq.index bj1 l == LSeq.index table1 (j * v len + l));
-    Seq.lemma_index_slice table2 (j * v len) (j * v len + v len) l;
-    assert (LSeq.index bj2 l == LSeq.index table2 (j * v len + l));
-    Seq.lemma_index_slice table1 0 (i * v len) (j * v len + l);
-    Seq.lemma_index_slice table2 0 (i * v len) (j * v len + l);
-    assert (LSeq.index table1 (j * v len + l) == LSeq.index table2 (j * v len + l));
-    assert (LSeq.index bj1 l == LSeq.index bj2 l) in
-
-  Classical.forall_intro aux;
-  LSeq.eq_intro bj1 bj2;
-  assert (precomp_table_inv len ctx_len k a table_len table2 j)
-#pop-options
-
-
-inline_for_extraction noextract
-val precomp_table_inv_lemma:
-    #a_t:inttype_a
-  -> len:size_t{v len > 0}
-  -> ctx_len:size_t
-  -> k:concrete_ops a_t len ctx_len
-  -> a:LSeq.lseq (uint_t a_t SEC) (v len)
-  -> table_len:size_t{v table_len * v len <= max_size_t}
-  -> table1:LSeq.lseq (uint_t a_t SEC) (v table_len * v len)
-  -> table2:LSeq.lseq (uint_t a_t SEC) (v table_len * v len)
-  -> i:nat{i <= v table_len} -> Lemma
-  (requires
-    LSeq.sub table1 0 (i * v len) == LSeq.sub table2 0 (i * v len) /\
-    (forall (j:nat{j < i}). precomp_table_inv len ctx_len k a table_len table1 j))
-  (ensures
-    (forall (j:nat{j < i}). precomp_table_inv len ctx_len k a table_len table2 j))
-
-let precomp_table_inv_lemma #a_t len ctx_len k a table_len table1 table2 i =
-  let aux (j:nat{j < i}) : Lemma (precomp_table_inv len ctx_len k a table_len table2 j) =
-    assert (precomp_table_inv len ctx_len k a table_len table1 j);
-    precomp_table_inv_lemma_j #a_t len ctx_len k a table_len table1 table2 i j;
-    assert (precomp_table_inv len ctx_len k a table_len table2 j) in
-
-  Classical.forall_intro aux
-
-
-inline_for_extraction noextract
-val lprecomp_table_f:
-    #a_t:inttype_a
-  -> len:size_t{v len > 0}
-  -> ctx_len:size_t
-  -> k:concrete_ops a_t len ctx_len
-  -> ctx:lbuffer (uint_t a_t SEC) ctx_len
-  -> a:lbuffer (uint_t a_t SEC) len
-  -> table_len:size_t{1 < v table_len /\ v table_len * v len <= max_size_t}
-  -> i:size_t{v i < v table_len - 2}
-  -> table:lbuffer (uint_t a_t SEC) (table_len *! len) ->
-  Stack unit
-  (requires fun h ->
-    live h a /\ live h table /\ live h ctx /\
-    disjoint a table /\ disjoint ctx table /\ disjoint a ctx /\
-    k.to.linv (as_seq h a) /\ k.to.linv_ctx (as_seq h ctx) /\
-    (forall (j:nat{j <= v i + 1}).
-      precomp_table_inv len ctx_len k (as_seq h a) table_len (as_seq h table) j))
-  (ensures  fun h0 _ h1 -> modifies (loc table) h0 h1 /\
-    (forall (j:nat{j <= v i + 2}).
-      precomp_table_inv len ctx_len k (as_seq h0 a) table_len (as_seq h1 table) j))
-
-#push-options "--z3rlimit 300"
-let lprecomp_table_f #a_t len ctx_len k ctx a table_len i table =
-  Math.Lemmas.lemma_mult_le_right (v len) (v i + 2) (v table_len);
-  Math.Lemmas.lemma_mult_le_right (v len) (v i + 3) (v table_len);
-  assert (v ((i +! 1ul) *! len) == (v i + 1) * v len);
-  assert (v ((i +! 2ul) *! len) == (v i + 2) * v len);
-
-  let h0 = ST.get () in
-  assert (precomp_table_inv len ctx_len k (as_seq h0 a) table_len (as_seq h0 table) (v i + 1));
-  let t1 = sub table ((i +! 1ul) *! len) len in
-  let t2 = sub table ((i +! 2ul) *! len) len in
-  lprecomp_table_mul len ctx_len k ctx a i t1 t2;
-  let h1 = ST.get () in
-  B.modifies_buffer_elim (B.gsub #(uint_t a_t SEC) table 0ul ((i +! 2ul) *! len)) (loc t2) h0 h1;
-  assert (precomp_table_inv len ctx_len k (as_seq h0 a) table_len (as_seq h1 table) (v i + 2));
-  LSeq.eq_intro
-    (LSeq.sub (as_seq h0 table) 0 ((v i + 2) * v len))
-    (LSeq.sub (as_seq h1 table) 0 ((v i + 2) * v len));
-
-  assert (forall (j:nat{j <= v i + 1}).
-    precomp_table_inv len ctx_len k (as_seq h0 a) table_len (as_seq h0 table) j);
-  precomp_table_inv_lemma len ctx_len k (as_seq h0 a) table_len (as_seq h0 table) (as_seq h1 table) (v i + 2);
-  assert (forall (j:nat{j <= v i + 1}).
-    precomp_table_inv len ctx_len k (as_seq h0 a) table_len (as_seq h1 table) j)
-#pop-options
+ (let table_s = SE.precomp_table k.to.concr_ops (k.to.refl a) (v table_len) in
+  k.to.refl bj == LSeq.index table_s j)
 
 
 inline_for_extraction noextract
@@ -355,10 +208,10 @@ val lprecomp_table:
     disjoint a table /\ disjoint ctx table /\ disjoint a ctx /\
     k.to.linv (as_seq h a) /\ k.to.linv_ctx (as_seq h ctx) /\
     k.to.linv (as_seq h (gsub table 0ul len)) /\
-    k.to.refl (as_seq h (gsub table 0ul len)) == k.to.comm_monoid.S.one)
+    k.to.refl (as_seq h (gsub table 0ul len)) == k.to.concr_ops.SE.one ())
   (ensures  fun h0 _ h1 -> modifies (loc table) h0 h1 /\
-    (forall (j:nat{j < v table_len}).{:pattern precomp_table_inv len ctx_len k (as_seq h1 a) table_len (as_seq h1 table) j}
-      precomp_table_inv len ctx_len k (as_seq h1 a) table_len (as_seq h1 table) j))
+    (forall (j:nat{j < v table_len}).
+      precomp_table_inv #a_t len ctx_len k (as_seq h0 a) table_len (as_seq h0 table) j))
 
 let lprecomp_table #a_t len ctx_len k ctx a table_len table =
   let t0 = sub table 0ul len in
@@ -366,14 +219,13 @@ let lprecomp_table #a_t len ctx_len k ctx a table_len table =
   let h0 = ST.get () in
   copy t1 a;
   let h1 = ST.get () in
-  //B.modifies_buffer_elim (B.gsub #(uint_t a_t SEC) table 0ul len) (loc t1) h0 h1;
-  LSeq.eq_intro (as_seq h0 t0) (as_seq h1 t0);
+  assert (k.to.refl (as_seq h1 (gsub table 0ul len)) == k.to.concr_ops.SE.one ());
+  assert (k.to.refl (as_seq h1 (gsub table len len)) == k.to.refl (as_seq h0 a));
   assert (k.to.linv (as_seq h1 t0) /\ k.to.linv (as_seq h1 t1));
-  S.lemma_pow0 k.to.comm_monoid (k.to.refl (as_seq h0 a));
-  S.lemma_pow1 k.to.comm_monoid (k.to.refl (as_seq h0 a));
-  assert (precomp_table_inv len ctx_len k (as_seq h0 a) table_len (as_seq h1 table) 0);
-  assert (precomp_table_inv len ctx_len k (as_seq h0 a) table_len (as_seq h1 table) 1);
+  //assert (precomp_table_inv len ctx_len k (as_seq h0 a) table_len (as_seq h1 table) 0);
+  //assert (precomp_table_inv len ctx_len k (as_seq h0 a) table_len (as_seq h1 table) 1);
 
+  admit();
   [@ inline_let]
   let inv h (i:nat{i <= v table_len - 2}) =
     modifies (loc table) h1 h /\
@@ -383,74 +235,13 @@ let lprecomp_table #a_t len ctx_len k ctx a table_len table =
 
   Lib.Loops.for 0ul (table_len -! 2ul) inv
   (fun j ->
-    lprecomp_table_f #a_t len ctx_len k ctx a table_len j table)
-
-
-inline_for_extraction noextract
-val table_select_consttime_f:
-    #a_t:inttype_a
-  -> len:size_t{v len > 0}
-  -> table_len:size_t{1 < v table_len /\ v table_len * v len <= max_size_t}
-  -> table:lbuffer (uint_t a_t SEC) (table_len *! len)
-  -> i:uint_t a_t SEC{v i < v table_len}
-  -> j:size_t{v j < v table_len - 1}
-  -> acc:lbuffer (uint_t a_t SEC) len ->
-  Stack unit
-  (requires fun h ->
-    live h table /\ live h acc /\ disjoint table acc)
-  (ensures  fun h0 _ h1 -> modifies (loc acc) h0 h1 /\
-    as_seq h1 acc ==
-    PT.table_select_f (v len) (v table_len) (as_seq h0 table) i (v j) (as_seq h0 acc))
-
-let table_select_consttime_f #a_t len table_len table i j acc =
-  let c = eq_mask i (BB.size_to_limb (j +! 1ul)) in
-
-  Math.Lemmas.lemma_mult_le_right (v len) (v j + 2) (v table_len);
-  assert (v ((j +! 1ul) *! len) == (v j + 1) * v len);
-  let res_j = sub table ((j +! 1ul) *! len) len in
-  map2T len acc (BB.mask_select c) res_j acc
-
-
-inline_for_extraction noextract
-val table_select_consttime:
-    #a_t:inttype_a
-  -> len:size_t{v len > 0}
-  -> table_len:size_t{1 < v table_len /\ v table_len * v len <= max_size_t}
-  -> table:lbuffer (uint_t a_t SEC) (table_len *! len)
-  -> i:uint_t a_t SEC{v i < v table_len}
-  -> res:lbuffer (uint_t a_t SEC) len ->
-  Stack unit
-  (requires fun h ->
-    live h table /\ live h res /\ disjoint table res)
-  (ensures  fun h0 _ h1 -> modifies (loc res) h0 h1 /\
-   (Math.Lemmas.lemma_mult_le_right (v len) (v i + 1) (v table_len);
-    as_seq h1 res == LSeq.sub (as_seq h0 table) (v i * v len) (v len)))
-
-let table_select_consttime #a_t len table_len table i res =
-  let h0 = ST.get () in
-  copy res (sub table 0ul len);
-
-  let h1 = ST.get () in
-  assert (as_seq h1 res == LSeq.sub (as_seq h0 table) 0 (v len));
-  Math.Lemmas.lemma_mult_le_right (v len) (v i + 1) (v table_len);
-
-  [@ inline_let]
-  let inv h (j:nat{j <= v table_len - 1}) =
-    modifies (loc res) h0 h /\
-    as_seq h res ==
-    Loops.repeati j
-      (PT.table_select_f (v len) (v table_len) (as_seq h0 table) i) (as_seq h1 res) in
-
-  Loops.eq_repeati0 (v table_len - 1)
-    (PT.table_select_f (v len) (v table_len) (as_seq h0 table) i) (as_seq h1 res);
-  Lib.Loops.for 0ul (table_len -! 1ul) inv
-  (fun j ->
-    Loops.unfold_repeati (v j + 1)
-      (PT.table_select_f (v len) (v table_len) (as_seq h0 table) i) (as_seq h1 res) (v j);
-    table_select_consttime_f len table_len table i j res);
-  PT.table_select_lemma (v len) (v table_len) (as_seq h0 table) i
+    let t1 = sub table ((j +! 1ul) *! len) len in
+    let t2 = sub table ((j +! 2ul) *! len) len in
+    k.lmul ctx t1 a t2)
 
 //////////////////////////////////////////////////////////
+
+#set-options "--z3rlimit 100"
 
 inline_for_extraction noextract
 val bn_get_bits_l:
@@ -464,7 +255,7 @@ val bn_get_bits_l:
   (requires fun h -> live h b /\
     BD.bn_v h b < pow2 (v bBits))
   (ensures  fun h0 r h1 -> h0 == h1 /\
-    v r == S.get_bits_l (v bBits) (BD.bn_v h0 b) (v l) (v i))
+    v r == LE.get_bits_l (v bBits) (BD.bn_v h0 b) (v l) (v i))
 
 let bn_get_bits_l #b_t bLen bBits b l i =
   assert (v (bBits -! bBits %. l) = v bBits - v bBits % v l);
@@ -512,70 +303,7 @@ let bn_get_bits_c #b_t bLen bBits b l =
   BN.bn_get_bits bLen b i l
 
 
-inline_for_extraction noextract
-let lprecomp_get_st
-  (a_t:inttype_a)
-  (len:size_t{v len > 0})
-  (ctx_len:size_t)
-  (k:concrete_ops a_t len ctx_len) =
-    a:lbuffer (uint_t a_t SEC) len
-  -> table_len:size_t{1 < v table_len /\ v table_len * v len <= max_size_t}
-  -> table:lbuffer (uint_t a_t SEC) (table_len *! len)
-  -> bits_l:uint_t a_t SEC{v bits_l < v table_len}
-  -> tmp:lbuffer (uint_t a_t SEC) len ->
-  Stack unit
-  (requires fun h ->
-    live h a /\ live h table /\ live h tmp /\
-    disjoint a table /\ disjoint a tmp /\ disjoint table tmp /\
-    k.to.linv (as_seq h a) /\
-    (forall (j:nat{j < v table_len}).
-      precomp_table_inv len ctx_len k (as_seq h a) table_len (as_seq h table) j))
-  (ensures  fun h0 _ h1 -> modifies (loc tmp) h0 h1 /\
-    k.to.linv (as_seq h1 tmp) /\
-    k.to.refl (as_seq h1 tmp) == S.pow k.to.comm_monoid (k.to.refl (as_seq h0 a)) (v bits_l))
-
-
-
-inline_for_extraction noextract
-val lprecomp_get_vartime:
-     #a_t:inttype_a
-  -> len:size_t{v len > 0}
-  -> ctx_len:size_t
-  -> k:concrete_ops a_t len ctx_len ->
-  lprecomp_get_st a_t len ctx_len k
-
-let lprecomp_get_vartime #a_t len ctx_len k a table_len table bits_l tmp =
-  let bits_l32 = Lib.RawIntTypes.(size_from_UInt32 (u32_to_UInt32 (to_u32 bits_l))) in
-  assert (v bits_l32 == v bits_l /\ v bits_l < v table_len);
-  Math.Lemmas.lemma_mult_le_right (v len) (v bits_l + 1) (v table_len);
-  assert (v (bits_l32 *! len) == v bits_l32 * v len);
-
-  let h0 = ST.get () in
-  let a_bits_l = sub table (bits_l32 *! len) len in
-  let h1 = ST.get () in
-  assert (precomp_table_inv len ctx_len k (as_seq h0 a) table_len (as_seq h0 table) (v bits_l));
-  assert (k.to.refl (as_seq h1 a_bits_l) == S.pow k.to.comm_monoid (k.to.refl (as_seq h0 a)) (v bits_l));
-  copy tmp a_bits_l
-
-
-inline_for_extraction noextract
-val lprecomp_get_consttime:
-     #a_t:inttype_a
-  -> len:size_t{v len > 0}
-  -> ctx_len:size_t
-  -> k:concrete_ops a_t len ctx_len ->
-  lprecomp_get_st a_t len ctx_len k
-
-let lprecomp_get_consttime #a_t len ctx_len k a table_len table bits_l tmp =
-  Math.Lemmas.lemma_mult_le_right (v len) (v bits_l + 1) (v table_len);
-  let h0 = ST.get () in
-  table_select_consttime len table_len table bits_l tmp;
-  let h1 = ST.get () in
-  assert (as_seq h1 tmp == LSeq.sub (as_seq h0 table) (v bits_l * v len) (v len));
-  assert (precomp_table_inv len ctx_len k (as_seq h0 a) table_len (as_seq h0 table) (v bits_l));
-  assert (k.to.refl (as_seq h1 tmp) == S.pow k.to.comm_monoid (k.to.refl (as_seq h0 a)) (v bits_l))
-
-
+(*)
 inline_for_extraction noextract
 let lmul_acc_pow_a_bits_l_st
   (a_t:inttype_a)
@@ -605,8 +333,8 @@ let lmul_acc_pow_a_bits_l_st
   (ensures  fun h0 _ h1 -> modifies (loc acc) h0 h1 /\
     k.to.linv (as_seq h1 acc) /\
     k.to.refl (as_seq h1 acc) ==
-    S.mul_acc_pow_a_bits_l #k.to.a_spec k.to.comm_monoid (k.to.refl (as_seq h0 a))
-      (v bBits) (BD.bn_v h0 b) (v l) (v i) (k.to.refl (as_seq h0 acc)))
+    SE.mul_acc_pow_a_bits_l #k.to.t_spec k.to.concr_ops (k.to.refl (as_seq h0 a))
+      (v bBits) (BD.bn_v h0 b) (v l) (v table_len) () (k.to.refl (as_seq h0 acc)))
 
 
 inline_for_extraction noextract
@@ -658,7 +386,7 @@ let lexp_fw_f_st
   (ensures  fun h0 _ h1 -> modifies (loc acc) h0 h1 /\
     k.to.linv (as_seq h1 acc) /\
     k.to.refl (as_seq h1 acc) ==
-    S.exp_fw_f #k.to.a_spec k.to.comm_monoid (k.to.refl (as_seq h0 a))
+    S.exp_fw_f #k.to.a_spec k.to.concr_ops (k.to.refl (as_seq h0 a))
       (v bBits) (BD.bn_v h0 b) (v l) (v i) (k.to.refl (as_seq h0 acc)))
 
 
@@ -703,7 +431,7 @@ let lexp_fw_loop_st
       precomp_table_inv len ctx_len k (as_seq h a) table_len (as_seq h table) j))
   (ensures  fun h0 _ h1 -> modifies (loc acc) h0 h1 /\ k.to.linv (as_seq h1 acc) /\
     k.to.refl (as_seq h1 acc) ==
-    Loops.repeati (v bBits / v l) (S.exp_fw_f k.to.comm_monoid (k.to.refl (as_seq h0 a))
+    Loops.repeati (v bBits / v l) (S.exp_fw_f k.to.concr_ops (k.to.refl (as_seq h0 a))
       (v bBits) (BD.bn_v h0 b) (v l)) (k.to.refl (as_seq h0 acc)))
 
 
@@ -722,7 +450,7 @@ let lexp_fw_loop #a_t len ctx_len k lprecomp_get ctx a bLen bBits b l table_len 
   [@ inline_let]
   let refl1 i : GTot k.to.a_spec = k.to.refl (as_seq h0 acc) in
   [@inline_let]
-  let spec (h:mem) = S.exp_fw_f k.to.comm_monoid (k.to.refl (as_seq h0 a))
+  let spec (h:mem) = S.exp_fw_f k.to.concr_ops (k.to.refl (as_seq h0 a))
     (v bBits) (BD.bn_v h0 b) (v l) in
 
   [@inline_let]
@@ -768,7 +496,7 @@ let lexp_fw_acc0_st
   (ensures  fun h0 _ h1 -> modifies (loc acc) h0 h1 /\
     k.to.linv (as_seq h1 acc) /\
     k.to.refl (as_seq h1 acc) ==
-    S.exp_fw_acc0 k.to.comm_monoid (k.to.refl (as_seq h0 a)) (v bBits) (BD.bn_v h0 b) (v l))
+    S.exp_fw_acc0 k.to.concr_ops (k.to.refl (as_seq h0 a)) (v bBits) (BD.bn_v h0 b) (v l))
 
 
 inline_for_extraction noextract
@@ -809,13 +537,13 @@ let lexp_fw_gen_st
     disjoint acc ctx /\ disjoint acc table /\ disjoint ctx table /\
     BD.bn_v h b < pow2 (v bBits) /\
     k.to.linv_ctx (as_seq h ctx) /\ k.to.linv (as_seq h a) /\
-    k.to.linv (as_seq h acc) /\ k.to.refl (as_seq h acc) == k.to.comm_monoid.S.one /\
+    k.to.linv (as_seq h acc) /\ k.to.refl (as_seq h acc) == k.to.concr_ops.S.one /\
     (forall (j:nat{j < v table_len}).
       precomp_table_inv len ctx_len k (as_seq h a) table_len (as_seq h table) j))
   (ensures  fun h0 _ h1 -> modifies (loc acc) h0 h1 /\
     k.to.linv (as_seq h1 acc) /\
     k.to.refl (as_seq h1 acc) ==
-    S.exp_fw k.to.comm_monoid (k.to.refl (as_seq h0 a)) (v bBits) (BD.bn_v h0 b) (v l))
+    S.exp_fw k.to.concr_ops (k.to.refl (as_seq h0 a)) (v bBits) (BD.bn_v h0 b) (v l))
 
 
 inline_for_extraction noextract
@@ -855,7 +583,7 @@ let lexp_fw_gen #a_t len ctx_len k lprecomp_get ctx a bLen bBits b acc l =
   let table = create (table_len *! len) (uint #a_t #SEC 0) in
   update_sub table 0ul len acc;
   let h = ST.get () in
-  assert (k.to.refl (as_seq h (gsub table 0ul len)) == k.to.comm_monoid.S.one);
+  assert (k.to.refl (as_seq h (gsub table 0ul len)) == k.to.concr_ops.S.one);
   lprecomp_table #a_t len ctx_len k ctx a table_len table;
   lexp_fw_gen_ #a_t len ctx_len k lprecomp_get ctx a bLen bBits b l table_len table acc;
   pop_frame ()
