code/bignum/Hacl.Impl.PrecompTable.fst
@@ -1,0 +1,115 @@
+module Hacl.Impl.PrecompTable
+
+open FStar.Mul
+
+open FStar.HyperStack
+open FStar.HyperStack.ST
+open FStar.Mul
+
+open Lib.IntTypes
+open Lib.Buffer
+
+module ST = FStar.HyperStack.ST
+module LSeq = Lib.Sequence
+module Loops = Lib.LoopCombinators
+
+module BB = Hacl.Bignum.Base
+module PT = Hacl.Spec.PrecompTable
+
+open Hacl.Spec.Bignum.Definitions
+
+#reset-options "--z3rlimit 50 --fuel 0 --ifuel 0"
+
+inline_for_extraction noextract
+val table_select_consttime_f:
+    #t:limb_t
+  -> len:size_t{v len > 0}
+  -> table_len:size_t{1 < v table_len /\ v table_len * v len <= max_size_t}
+  -> table:lbuffer (uint_t t SEC) (table_len *! len)
+  -> i:uint_t t SEC{v i < v table_len}
+  -> j:size_t{v j < v table_len - 1}
+  -> acc:lbuffer (uint_t t SEC) len ->
+  Stack unit
+  (requires fun h ->
+    live h table /\ live h acc /\ disjoint table acc)
+  (ensures  fun h0 _ h1 -> modifies (loc acc) h0 h1 /\
+    as_seq h1 acc ==
+    PT.table_select_f (v len) (v table_len) (as_seq h0 table) i (v j) (as_seq h0 acc))
+
+let table_select_consttime_f #t len table_len table i j acc =
+  let c = eq_mask i (BB.size_to_limb (j +! 1ul)) in
+
+  Math.Lemmas.lemma_mult_le_right (v len) (v j + 2) (v table_len);
+  assert (v ((j +! 1ul) *! len) == (v j + 1) * v len);
+  let res_j = sub table ((j +! 1ul) *! len) len in
+  map2T len acc (BB.mask_select c) res_j acc
+
+
+inline_for_extraction noextract
+val table_select_consttime:
+    #t:limb_t
+  -> len:size_t{v len > 0}
+  -> table_len:size_t{1 < v table_len /\ v table_len * v len <= max_size_t}
+  -> table:lbuffer (uint_t t SEC) (table_len *! len)
+  -> i:uint_t t SEC{v i < v table_len}
+  -> res:lbuffer (uint_t t SEC) len ->
+  Stack unit
+  (requires fun h ->
+    (v i + 1) * v len <= v table_len * v len /\
+    live h table /\ live h res /\ disjoint table res)
+  (ensures  fun h0 _ h1 -> modifies (loc res) h0 h1 /\
+    as_seq h1 res == LSeq.sub (as_seq h0 table) (v i * v len) (v len))
+
+let table_select_consttime #t len table_len table i res =
+  let h0 = ST.get () in
+  copy res (sub table 0ul len);
+
+  let h1 = ST.get () in
+  assert (as_seq h1 res == LSeq.sub (as_seq h0 table) 0 (v len));
+
+  [@ inline_let]
+  let inv h (j:nat{j <= v table_len - 1}) =
+    modifies (loc res) h0 h /\
+    as_seq h res ==
+    Loops.repeati j
+      (PT.table_select_f (v len) (v table_len) (as_seq h0 table) i) (as_seq h1 res) in
+
+  Loops.eq_repeati0 (v table_len - 1)
+    (PT.table_select_f (v len) (v table_len) (as_seq h0 table) i) (as_seq h1 res);
+  Lib.Loops.for 0ul (table_len -! 1ul) inv
+  (fun j ->
+    Loops.unfold_repeati (v j + 1)
+      (PT.table_select_f (v len) (v table_len) (as_seq h0 table) i) (as_seq h1 res) (v j);
+    table_select_consttime_f len table_len table i j res);
+  PT.table_select_lemma (v len) (v table_len) (as_seq h0 table) i
+
+
+inline_for_extraction noextract
+let table_get_st (t:limb_t) (len:size_t{v len > 0}) =
+    table_len:size_t{1 < v table_len /\ v table_len * v len <= max_size_t}
+  -> table:lbuffer (uint_t t SEC) (table_len *! len)
+  -> i:uint_t t SEC{v i < v table_len}
+  -> tmp:lbuffer (uint_t t SEC) len ->
+  Stack unit
+  (requires fun h ->
+    (v i + 1) * v len <= v table_len * v len /\
+    live h table /\ live h tmp /\ disjoint table tmp)
+  (ensures  fun h0 _ h1 -> modifies (loc tmp) h0 h1 /\
+    as_seq h1 tmp == LSeq.sub (as_seq h0 table) (v i * v len) (v len))
+
+
+inline_for_extraction noextract
+val table_get_vartime: #t:limb_t -> len:size_t{v len > 0} -> table_get_st t len
+let table_get_vartime #t len table_len table i tmp =
+  let i32 = Lib.RawIntTypes.(size_from_UInt32 (u32_to_UInt32 (to_u32 i))) in
+  assert (v i32 == v i /\ v i < v table_len);
+  assert (v (i32 *! len) == v i32 * v len);
+
+  let a_i = sub table (i32 *! len) len in
+  copy tmp a_i
+
+
+inline_for_extraction noextract
+val table_get_consttime: #t:limb_t -> len:size_t{v len > 0} -> table_get_st t len
+let table_get_consttime #a_t len table_len table bits_l tmp =
+  table_select_consttime len table_len table bits_l tmp
