specs/Spec.Exponentiation.fsti
@@ -1,0 +1,196 @@
+module Spec.Exponentiation
+
+open FStar.Mul
+
+open Lib.IntTypes
+open Lib.Sequence
+
+module S = Lib.Exponentiation
+module Loops = Lib.LoopCombinators
+
+#set-options "--z3rlimit 50 --fuel 0 --ifuel 0"
+
+inline_for_extraction
+class to_cm (t:Type) = {
+  a_spec: Type;
+  cm: S.comm_monoid a_spec;
+  refl: x:t -> a_spec;
+  }
+
+
+inline_for_extraction
+let one_st (t:Type) (to:to_cm t) = unit -> Pure t
+  (requires True)
+  (ensures  fun one ->
+    to.refl one == to.cm.S.one)
+
+
+inline_for_extraction
+let mul_st (t:Type) (to:to_cm t) = x:t -> y:t -> Pure t
+  (requires True)
+  (ensures  fun xy ->
+    to.refl xy == to.cm.S.mul (to.refl x) (to.refl y))
+
+
+inline_for_extraction
+let sqr_st (t:Type) (to:to_cm t) = x:t -> Pure t
+  (requires True)
+  (ensures  fun xy ->
+    to.refl xy == to.cm.S.mul (to.refl x) (to.refl x))
+
+
+inline_for_extraction
+class concrete_ops (t:Type) = {
+  to: to_cm t;
+  one: one_st t to;
+  mul: mul_st t to;
+  sqr: sqr_st t to;
+  }
+
+
+let exp_rl_f (#t:Type) (k:concrete_ops t)
+  (bBits:nat) (b:nat{b < pow2 bBits})
+  (i:nat{i < bBits}) ((acc, c) : tuple2 t t) : tuple2 t t
+ =
+  let acc = if (S.get_ith_bit bBits b i = 0) then acc else k.mul acc c in
+  let c = k.sqr c in
+  (acc, c)
+
+
+let exp_rl (#t:Type) (k:concrete_ops t) (a:t) (bBits:nat) (b:nat{b < pow2 bBits}) : t =
+  let one = k.one () in
+  let (acc, c) = Loops.repeati bBits (exp_rl_f k bBits b) (one, a) in
+  acc
+
+
+val exp_rl_lemma: #t:Type -> k:concrete_ops t -> a:t -> bBits:nat -> b:nat{b < pow2 bBits} ->
+  Lemma (k.to.refl (exp_rl k a bBits b) == S.exp_rl k.to.cm (k.to.refl a) bBits b)
+
+
+let exp_mont_ladder_swap_f (#t:Type) (k:concrete_ops t)
+  (bBits:nat) (b:nat{b < pow2 bBits})
+  (i:nat{i < bBits}) ((r0, r1, privbit) : tuple3 t t nat) : tuple3 t t nat
+ =
+  let bit = S.get_ith_bit bBits b (bBits - 1 - i) in
+  let sw = (bit + privbit) % 2 in
+  let r0, r1 = S.cswap sw r0 r1 in
+  let r0, r1 = (k.sqr r0, k.mul r1 r0) in
+  (r0, r1, bit)
+
+
+let exp_mont_ladder_swap (#t:Type) (k:concrete_ops t) (a:t) (bBits:nat) (b:nat{b < pow2 bBits}) : t =
+  let (r0, r1, sw) = Loops.repeati bBits (exp_mont_ladder_swap_f k bBits b) (one (), a, 0) in
+  let (r0, r1) = S.cswap sw r0 r1 in
+  r0
+
+
+val exp_mont_ladder_swap_lemma: #t:Type -> k:concrete_ops t -> a:t -> bBits:nat -> b:nat{b < pow2 bBits} ->
+  Lemma (k.to.refl (exp_mont_ladder_swap k a bBits b) == S.exp_mont_ladder_swap k.to.cm (k.to.refl a) bBits b)
+
+
+let exp_pow2 (#t:Type) (k:concrete_ops t) (a:t) (b:nat) : t =
+  Loops.repeat b k.sqr a
+
+
+val exp_pow2_lemma: #t:Type -> k:concrete_ops t -> a:t -> b:nat ->
+  Lemma (k.to.refl (exp_pow2 k a b) == S.exp_pow2 k.to.cm (k.to.refl a) b)
+
+
+let precomp_table_f (#t:Type0) (k:concrete_ops t) (a:t)
+  (table_len:size_nat{1 < table_len}) (i:nat{i < table_len - 2}) (table:lseq t table_len) : lseq t table_len
+ =
+  table.[i + 2] <- k.mul table.[i + 1] a
+
+
+let precomp_table (#t:Type0) (k:concrete_ops t) (a:t) (table_len:size_nat{1 < table_len}) : lseq t table_len =
+  let table = create table_len (k.one ()) in
+  let table = table.[0] <- one () in
+  let table = table.[1] <- a in
+
+  Loops.repeati (table_len - 2) (precomp_table_f k a table_len) table
+
+
+let exp_fw_acc0 (#t:Type0) (k:concrete_ops t) (a:t)
+  (bBits:nat) (b:nat{b < pow2 bBits}) (l:pos{bBits % l <> 0})
+  (table_len:size_nat{table_len == pow2 l}) (table:lseq t table_len) : t
+ =
+  let bits_c = S.get_ith_lbits bBits b (bBits / l * l) l in
+  table.[bits_c]
+
+
+let mul_acc_pow_a_bits_l (#t:Type) (k:concrete_ops t) (a:t)
+  (bBits:nat) (b:nat{b < pow2 bBits}) (l:pos)
+  (table_len:size_nat{table_len == pow2 l}) (table:lseq t table_len)
+  (i:nat{i < bBits / l}) (acc:t) : t
+ =
+  let bits_l = S.get_bits_l bBits b l i in
+  k.mul acc table.[bits_l]
+
+
+let exp_fw_f (#t:Type) (k:concrete_ops t) (a:t)
+  (bBits:nat) (b:nat{b < pow2 bBits}) (l:pos)
+  (table_len:size_nat{table_len == pow2 l}) (table:lseq t table_len)
+  (i:nat{i < bBits / l}) (acc:t) : t
+ =
+  let acc1 = exp_pow2 k acc l in
+  mul_acc_pow_a_bits_l k a bBits b l table_len table i acc1
+
+
+let exp_fw (#t:Type) (k:concrete_ops t) (a:t) (bBits:nat) (b:nat{b < pow2 bBits}) (l:pos{l < 32}) : t =
+  Math.Lemmas.pow2_lt_compat 32 l;
+  Math.Lemmas.pow2_lt_compat l 0;
+  let table_len : size_nat = pow2 l in
+  let table = precomp_table k a table_len in
+
+  let acc0 = if bBits % l = 0 then one () else exp_fw_acc0 k a bBits b l table_len table in
+  Loops.repeati (bBits / l) (exp_fw_f k a bBits b l table_len table) acc0
+
+
+val exp_fw_lemma: #t:Type -> k:concrete_ops t -> a:t -> bBits:nat -> b:nat{b < pow2 bBits} -> l:pos{l < 32} ->
+  Lemma (k.to.refl (exp_fw k a bBits b l) == S.exp_fw k.to.cm (k.to.refl a) bBits b l)
+
+
+let exp_double_fw_acc0 (#t:Type) (k:concrete_ops t)
+  (a1:t) (bBits:nat) (b1:nat{b1 < pow2 bBits})
+  (a2:t) (b2:nat{b2 < pow2 bBits}) (l:pos{bBits % l <> 0})
+  (table_len:size_nat{table_len == pow2 l}) (table1:lseq t table_len) (table2:lseq t table_len) : t
+ =
+  let acc_a1 = exp_fw_acc0 k a1 bBits b1 l table_len table1 in
+  let acc_a2 = exp_fw_acc0 k a2 bBits b2 l table_len table2 in
+  k.mul acc_a1 acc_a2
+
+
+let exp_double_fw_f (#t:Type) (k:concrete_ops t)
+  (a1:t) (bBits:nat) (b1:nat{b1 < pow2 bBits})
+  (a2:t) (b2:nat{b2 < pow2 bBits}) (l:pos)
+  (table_len:size_nat{table_len == pow2 l}) (table1:lseq t table_len) (table2:lseq t table_len)
+  (i:nat{i < bBits / l}) (acc:t) : t
+ =
+  let acc1 = exp_fw_f k a1 bBits b1 l table_len table1 i acc in
+  mul_acc_pow_a_bits_l k a2 bBits b2 l table_len table2 i acc1
+
+
+let exp_double_fw (#t:Type) (k:concrete_ops t)
+  (a1:t) (bBits:nat) (b1:nat{b1 < pow2 bBits})
+  (a2:t) (b2:nat{b2 < pow2 bBits}) (l:pos{l < 32}) : t
+ =
+
+  Math.Lemmas.pow2_lt_compat 32 l;
+  Math.Lemmas.pow2_lt_compat l 0;
+  let table_len : size_nat = pow2 l in
+  let table1 = precomp_table k a1 table_len in
+  let table2 = precomp_table k a2 table_len in
+
+  let acc0 =
+    if bBits % l = 0 then one ()
+    else exp_double_fw_acc0 k a1 bBits b1 a2 b2 l table_len table1 table2 in
+
+  Loops.repeati (bBits / l)
+    (exp_double_fw_f k a1 bBits b1 a2 b2 l table_len table1 table2) acc0
+
+
+val exp_double_fw_lemma: #t:Type -> k:concrete_ops t
+  -> a1:t -> bBits:nat -> b1:nat{b1 < pow2 bBits}
+  -> a2:t -> b2:nat{b2 < pow2 bBits} -> l:pos{l < 32} ->
+  Lemma (k.to.refl (exp_double_fw k a1 bBits b1 a2 b2 l) ==
+    S.exp_double_fw k.to.cm (k.to.refl a1) bBits b1 (k.to.refl a2) b2 l)
